\documentclass{article}
\usepackage[utf8]{inputenc}
\usepackage[english]{babel}
\usepackage{amsthm}
\usepackage{amssymb}

\newtheorem*{claim}{Claim}
\renewcommand\qedsymbol{$\blacksquare$} 
\begin{document}
\begin{claim}
  For any integer $n$ \(\geq\) 1, \(2^1+2^2+2^3+ ... +2^n = 2^{n+1}-2\).
\end{claim}
 
\begin{proof}
By induction. Base case: Let n = 1. Then \(2^1=2^{1+1}-2\). The right hand side evalutes 
  to 4 - 2, which is equal to the left hand side 2. From Inductive Hypothesis: 
  assume claim holds for some $n$. We will show it holds for \(n+1\).
  \(2^1+...+2^n+2^{n+1} = 2^{n+1}-2+2^{n+1}\). Combining like terms, we get
  \(2^{n+2}-2 = 2^{(n+1)+1} - 2\), which is what we were looking for.

\end{proof}
\end{document}


