\documentclass{article}
\usepackage[utf8]{inputenc}
\usepackage[english]{babel}
\usepackage{amsthm}
\usepackage{amssymb}

\newtheorem{lemma}{Lemma}
\renewcommand\qedsymbol{$\blacksquare$} 
\begin{document}
\begin{lemma}
Prove that if $n$ is even, \((-1)^n = 1\).
\end{lemma}
 
\begin{proof}
Let n be an integer, and assume it is even. By definition, there exists an integer k such that n = 2k.
  Hence, \((-1)^n = (-1)^{2k} = (-1^2)^k\). \((-1)^2 = 1\), and 1 to the power of any number k equates to 1.  
\end{proof}
\end{document}


