\documentclass{article}
\usepackage[utf8]{inputenc}
\usepackage[english]{babel}
\usepackage{amsthm}
\usepackage{amssymb}

\author{Kevin Martin\\ CIS675 - Syracuse University}
\title{Exercise 2.2}

\newtheorem{claim}{Claim}
\renewcommand\qedsymbol{$\blacksquare$} 
\begin{document}
\maketitle
\begin{claim}
  T(0) = 1, T(1) = 0, T(n) = 2 * T(n-2)\\
  has the solution T(n) = \(2^{n\over 2}*(1-(n\%2))\).
\end{claim}
 
\begin{proof}
Proof by induction. Base case: n = 0.\\
  Base case: let n=0, T(0) = \(2^{0/2}\)*(1-(0\%2))=\(2^0\)*(1-0) = T(0), and T(0)=1\\
  Second base case: let n=1, T(1)=\(2^{1\over 2}\)*)1-(1\%2))=\(2^{1\over 2}\)*(1-1)=\(2^{1/2}\)*0=0//
  Assume that the claim holds for some even n=2*u, T(n)=\(2^u\)\\
  IH: show the claim holds for (n+2)=2*(u+1)\\
  T(2*u+2)=2*T(2*u)\\
        = 2 * \(2^{2*{u\over 2}}\) * (1-((2*u)\%2))\\
        = 2 * \(2^{u}\) *(1-0) = (2*\(2^{u}\))*1 = \(2^{u+1}\)

\end{proof}

\begin{claim}
  T(0) = 0,T(n) = T(n-1) + n
\end{claim}
 
\begin{proof}
Proof by induction. Base case: n = 0.\\
  T(0) = 0. 1 +...+ 0 = 0. Base case holds\\
  IH: T(n) = 1+2+...+ n. Show claim holds for n+1:\\
  T(n+1) = T(n) + n + 1 = 1 + 2 + ... + n + (n + 1)
\end{proof}

\begin{claim}
  T(0) = 0, T(n) = T(n-1) * n
\end{claim}
 
\begin{proof}
  Proof by induction. Base case: n = 0, T(0) = 0.\\
  IH: Assume for some n that T(n) = 0. Show that T(n + 1) = 0.\\
  T(n+1) = T(n) * (n+1) = 0
\end{proof}
\begin{claim}
  T(1) = 1, T(n) = 2 * T(n/2) (Assume n is a power of 2.)
\end{claim}
 
\begin{proof}
\end{proof}
\begin{claim}
  T(0) = 1, T(1) = 2, T(n) = 2 * T(n-2)
\end{claim}
 
\begin{proof}
\end{proof}

\begin{claim}
  T(0) = -1, T(n) = \((T(n-1)^2\)
\end{claim}
 
\begin{proof}
\end{proof}

\end{document}


